wip end2end_lightbulb; cannot unify Naive word and Kami word

end2end/src/End2EndLightbulb.v
@@ -1,15 +1,20 @@
 Require Import Coq.ZArith.ZArith.
 Require Import Coq.Strings.String.
 Require Import Coq.Lists.List. Import ListNotations.
+Require Import coqutil.Word.Interface.
 Require Import coqutil.Map.Interface.
 Require Import end2end.End2EndPipeline.
 Require Import bedrock2.Syntax.
 Require Import bedrock2.Examples.lightbulb.
+Require Import bedrock2.TracePredicate. Import TracePredicateNotations.
 Require Import compiler.examples.integration.
 Require Import compiler.ProgramSpec.
+Require Import compiler.MemoryLayout.
 
 Open Scope Z_scope.
 Open Scope string_scope.
+
+Axiom TODO: False.
 
 Definition instrMemSizeLg: Z := 10. (* TODO is this enough? *)
 Definition dataMemSize: Z := 4096.
@@ -20,40 +25,86 @@ Definition funnamesList: list string.
   end.
 Defined.
 
+Definition funimplsMap: Semantics.env.
+  match type of link_lightbulb with
+  | spec_of_iot ?L =>
+    let keys := eval cbv in (List.map fst L) in
+    let values := eval cbv in (List.map snd L) in
+    let o := eval cbv in (@map.of_list _ _ Semantics.env keys values) in
+    lazymatch o with
+    | Some ?m => exact m
+    end
+  end.
+Defined.
+
 Definition buffer_addr: Z. Admitted.
 
 (* TODO is it ok to overwrite a register with "res"? *)
 Definition loopbody := @cmd.call Semantics.syntax ["res"] "iot" [expr.literal buffer_addr].
 
-Fail Check {|
+Definition prog := {|
   funnames := funnamesList;
-  init_code := cmd.skip;
+  funimpls := funimplsMap;
+  init_code := @cmd.skip Semantics.syntax;
   loop_body := @cmd.call Semantics.syntax ["res"] "iot" [expr.literal buffer_addr];
-
 |}.
 
-(*
-Definition prog: Program := {|
-  funnames := functionNames;
-  funimpls := Interface.map.of_list
-  init_code :=
-  loop_body :=
+Definition traceOfOneInteraction: list (lightbulb_spec.OP Semantics.word) -> Prop :=
+  (existsl (fun bytes => lightbulb_spec.lan9250_recv _ _ bytes)) |||
+  (lightbulb_spec.lan9250_recv_no_packet _ _) |||
+  (lightbulb_spec.lan9250_recv_packet_too_long _ _) |||
+  (any +++ (lightbulb_spec.spi_timeout _)).
 
-Definition spec
-Definition ml
-Definition mlOk
-Definition memInit
-Definition instrMemSizeLg_agrees_with_ml
+Definition goodHlTrace: list (lightbulb_spec.OP Semantics.word) -> Prop :=
+  traceOfOneInteraction ^*.
 
-*)
+Definition spec: ProgramSpec := {|
+  datamem_start := match TODO with end;
+  datamem_pastend := match TODO with end;
+  goodTrace iol := exists ioh, SPI.mmio_trace_abstraction_relation ioh iol /\
+                               goodHlTrace ioh;
+  isReady t m l := exists buf R,
+    (Separation.sep (Array.array Scalars.scalar8 (word.of_Z 1) (word.of_Z buffer_addr) buf) R) m /\
+    length buf = 1520%nat;
+|}.
+
+Definition ml: MemoryLayout 32. Admitted.
+
+Lemma mlOk: MemoryLayoutOk ml.
+Proof.
+  constructor.
+Admitted.
+
+Definition memInit: SC.MemInit (BinIntDef.Z.to_nat Semantics.width) IsaRv32.rv32DataBytes.
+Admitted.
+
+Lemma instrMemSizeLg_agrees_with_ml:
+  word.sub (code_pastend ml) (code_start ml) = word.of_Z instrMemSizeLg.
+Admitted.
+
+Goal @Naive.rep 32 = Word.word 32.
+  (* TODO does not hold: bedrock2 separation logic word <> kami word !! *)
+Abort.
 
 Lemma end2end_lightbulb: False.
 Proof.
   pose proof link_lightbulb as P.
   unfold spec_of_iot in *.
 
-
   pose proof @end2end as Q.
   specialize_first Q integration.mapops.
+
+  Fail specialize Q with (prog := prog).
+
+(*
+ instrMemSizeLg
+ dataMemSize
+ prog
+ spec
+ ml
+ mlOk
+ memInit
+ instrMemSizeLg_agrees_with_ml
+*)
 
 Abort.
